Concurrent example, including parallel allocation

examples/lowstar_concurrent/Test.Par.fst
@@ -39,19 +39,82 @@ let read_write_with_sharing () : RST unit
   let x, y = par 
     (fun _ -> A.array_resource b <*> A.array_resource b1)
     (fun () -> A.index b 0ul) (fun () -> A.index b1 1ul) in
-  // let x, y = par (A.array_resource b) (A.array_resource b1)
-  //   #_ #_
-  //   #(fun _ -> A.array_resource b) #(fun _ -> A.array_resource b1)
-  //   #_ #_ #_ #_
-  //   (fun () -> A.index b 0ul) (fun () -> A.index b1 1ul) in
-  // let x1 =
-  //   RST.rst_frame
-  //     (R.(A.array_resource b <*> A.array_resource b1))
-  //     (fun _ -> R.(A.array_resource b <*> A.array_resource b1))
-  //     (fun _ ->
-  //       A.index b 0ul
-  //     )
-  // in
-  // admit();
+  let x, y = par 
+    (fun _ -> A.array_resource b <*> A.array_resource b1)
+    (fun () -> A.index b 0ul) (fun () -> A.index b1 1ul) in
+  let x1 =
+    rst_frame
+      ((A.array_resource b <*> A.array_resource b1))
+      (fun _ -> (A.array_resource b <*> A.array_resource b1))
+      (fun _ ->
+        A.index b 0ul
+      )
+  in
   A.merge b b1;
   A.free b
+
+let parallel_alloc () : RST unit
+  (empty_resource)
+  (fun _ -> empty_resource)
+  (fun _ -> True)
+  (fun _ _ _ -> True)
+  =
+  // Need those to conclude that empty_resource ~= empty_resource <*> empty_resource
+  reveal_empty_resource();
+  reveal_star();
+  reveal_rst_inv();
+  reveal_modifies();
+  let h0 = HST.get() in
+  // Allocates in parallel 
+  let b1, b2 = par 
+    (fun (x, y) -> A.array_resource x <*> A.array_resource y)
+    (fun () -> A.alloc 2ul 2ul) (fun () -> A.alloc 2ul 2ul) in
+  let res0 = empty_resource in
+  let res1 = A.array_resource b1 <*> A.array_resource b2 in
+  let h1 = HST.get() in
+  // This explicit modifies is needed to trigger modifies_trans. Why?
+  assert (modifies res0 res1 h0 h1);
+  let x1 =
+    rst_frame
+      ((A.array_resource b1 <*> A.array_resource b2))
+      (fun _ -> (A.array_resource b1 <*> A.array_resource b2))
+      (fun _ ->
+        A.index b1 0ul
+      )
+  in
+  // We know the contents of each array after parallel allocation
+  assert (x1 == 2ul);
+  let _, x3 =
+    par (fun _ -> A.array_resource b1 <*> A.array_resource b2)
+      (fun _ -> A.upd b1 0ul 0ul) (fun () -> A.index b2 0ul) in
+  let x2 =
+    rst_frame
+      ((A.array_resource b1 <*> A.array_resource b2))
+      (fun _ -> (A.array_resource b1 <*> A.array_resource b2))
+      (fun _ ->
+        A.index b1 0ul
+      )
+  in
+  // We can modify just one array...
+  assert (x2 == 0ul);
+  let x3 =
+    rst_frame
+      ((A.array_resource b1 <*> A.array_resource b2))
+      (fun _ -> (A.array_resource b1 <*> A.array_resource b2))
+      (fun _ ->
+        A.index b2 0ul
+      )
+  in
+  // and we still know that the other one was unmodified (since it's starred)
+  assert (x3 == 2ul);
+
+  // We can also do the free in parallel if we want
+  // let _ = par (fun _ -> empty_resource <*> empty_resource)
+  //   (fun () -> A.free b1) (fun () -> A.free b2) in
+  rst_frame
+      ((A.array_resource b1 <*> A.array_resource b2))
+      (fun _ -> A.array_resource b2)
+      (fun _ ->
+        A.free b1
+      );
+  A.free b2
